Give more parameters to sepcomp_rel (WIP).

sepcomp/common/Language.v
@@ -50,13 +50,49 @@ Structure EF (sigT:Sig): Type := mkEF {
   EF_sig: forall (ef:EF_carrier), sigT
 }.
 
+Structure EquivalentType (A B:Type) := mkEquivalentType {
+  AtoB: forall (a:A), B;
+  BtoA: forall (b:B), A;
+  HABA: forall a, BtoA (AtoB a) = a;
+  HBAB: forall b, AtoB (BtoA b) = b
+}.
+
+Lemma EquivalentType_AtoB_inj
+      A B (E:EquivalentType A B)
+      a1 a2 (H: E.(AtoB) a1 = E.(AtoB) a2):
+  a1 = a2.
+Proof.
+  rewrite <- (HABA E a1), <- (HABA E a2).
+  rewrite H. auto.
+Qed.
+
+Lemma EquivalentType_AtoB_sur
+      A B (E:EquivalentType A B)
+      b:
+  exists a, E.(AtoB) a = b.
+Proof. exists (E.(BtoA) b). apply HBAB. Qed.
+
+Lemma EquivalentType_BtoA_inj
+      A B (E:EquivalentType A B)
+      b1 b2 (H: E.(BtoA) b1 = E.(BtoA) b2):
+  b1 = b2.
+Proof.
+  rewrite <- (HBAB E b1), <- (HBAB E b2).
+  rewrite H. auto.
+Qed.
+
+Lemma EquivalentType_BtoA_sur
+      A B (E:EquivalentType A B)
+      a:
+  exists b, E.(BtoA) b = a.
+Proof. exists (E.(AtoB) a). apply HABA. Qed.
+
 Structure Fundef (sigT:Sig) (fT:F sigT) (efT:EF sigT) := mkFundef {
   Fundef_carrier :> Type;
-  Fundef_dec: forall (fd:Fundef_carrier), fT + efT;
-  HFundef_dec_inj: forall fd1 fd2 (Hfd: Fundef_dec fd1 = Fundef_dec fd2), fd1 = fd2;
+  Fundef_equiv :> EquivalentType Fundef_carrier (fT + efT);
   Fundef_sig :=
     fun fd =>
-      match Fundef_dec fd with
+      match Fundef_equiv.(AtoB) fd with
         | inl f => fT.(F_sig) f
         | inr ef => efT.(EF_sig) ef
       end
@@ -76,50 +112,6 @@ Structure Language: Type := mkLanguage {
   globdefT := AST.globdef fundefT vT;
   progT := AST.program fundefT vT
 }.
-
-Structure Language_ext: Type := mkLanguage_ext {
-  lang :> Language;
-
-  stateT: Type;
-  contT: Type;
-  mkCallstate: forall (cont:contT) (fd:lang.(fundefT)) (args:list val) (m:mem), stateT;
-  mkReturnstate: forall (cont:contT) (v:val) (m:mem), stateT;
-  empty_cont: contT;
-
-  step: forall (ge:Genv.t lang.(fundefT) lang.(vT)) (state1:stateT) (evt:Events.trace) (state2:stateT), Prop;
-  signature_main: lang.(sigT);
-  initial_state := fun (p:lang.(progT)) (state:stateT) =>
-                     exists b f m0,
-                       let ge := Genv.globalenv p in
-                       Genv.init_mem p = Some m0 /\
-                       Genv.find_symbol ge p.(prog_main) = Some b /\
-                       Genv.find_funct_ptr ge b = Some f /\
-                       lang.(fundefT).(Fundef_sig) f = signature_main /\
-                       state = (mkCallstate empty_cont f nil m0);
-  final_state := fun (state:stateT) (r:int) =>
-                   exists m,
-                     state = mkReturnstate empty_cont (Vint r) m;
-  semantics := fun (p:lang.(progT)) =>
-                 Semantics step (initial_state p) final_state (Genv.globalenv p);
-
-  Hfinal_not_progress: forall v m,
-                         ~ exists ge evt state', step ge (mkReturnstate empty_cont v m) evt state';
-  Hfinal_not_call: forall v m1,
-                     ~ exists cont fd args m2, mkReturnstate empty_cont v m1 = mkCallstate cont fd args m2;
-  HmkReturnstate_inj: forall cont1 v1 m1 cont2 v2 m2 (H: mkReturnstate cont1 v1 m1 = mkReturnstate cont2 v2 m2),
-                        cont1 = cont2 /\ v1 = v2 /\ m1 = m2
-}.
-
-Lemma initial_state_unique lang p s1 s2
-      (H1: lang.(initial_state) p s1)
-      (H2: lang.(initial_state) p s2):
-  s1 = s2.
-Proof.
-  destruct H1 as [b [f [m0 [Hm0 [Hb [Hf [Hsig ?]]]]]]]. subst.
-  destruct H2 as [b' [f' [m0' [Hm0' [Hb' [Hf' [Hsig' ?]]]]]]]. subst.
-  rewrite Hm0 in Hm0'. inv Hm0'. rewrite Hb in Hb'. inv Hb'. rewrite Hf in Hf'. inv Hf'.
-  auto.
-Qed.
 
 (** Canonical Structures *)
 
@@ -149,251 +141,83 @@ Canonical Structure EF_external_function: EF Sig_signature :=
        ef_sig.
 
 Program Canonical Structure Fundef_C: Fundef F_C EF_external_function_ext :=
-  mkFundef F_C EF_external_function_ext
-           (fun fd =>
-              match fd with
-                | Csyntax.Internal f => inl f
-                | Csyntax.External ef targs tres cc => inr (ef, targs, tres, cc)
-              end) _.
-Next Obligation. destruct fd1, fd2; inv Hfd; auto. Qed.
+  @mkFundef _ F_C EF_external_function_ext Csyntax.fundef
+            (mkEquivalentType
+               (fun fd =>
+                  match fd with
+                    | Csyntax.Internal f => inl f
+                    | Csyntax.External ef targs tres cc => inr (ef, targs, tres, cc)
+                  end)
+               (fun fd =>
+                  match fd with
+                    | inl f => Csyntax.Internal f
+                    | inr (ef, targs, tres, cc) => Csyntax.External ef targs tres cc
+                  end)
+               _ _).
+Next Obligation. destruct a; auto. Qed.
+Next Obligation. destruct b; auto. destruct e. destruct p. destruct p. auto. Qed.
 Program Canonical Structure Fundef_Clight: Fundef F_Clight EF_external_function_ext :=
-  mkFundef F_Clight EF_external_function_ext
-           (fun fd =>
-              match fd with
-                | Clight.Internal f => inl f
-                | Clight.External ef targs tres cc => inr (ef, targs, tres, cc)
-              end) _.
-Next Obligation. destruct fd1, fd2; inv Hfd; auto. Qed.
+  @mkFundef _ F_Clight EF_external_function_ext Clight.fundef
+            (mkEquivalentType
+               (fun fd =>
+                  match fd with
+                    | Clight.Internal f => inl f
+                    | Clight.External ef targs tres cc => inr (ef, targs, tres, cc)
+                  end)
+               (fun fd =>
+                  match fd with
+                    | inl f => Clight.Internal f
+                    | inr (ef, targs, tres, cc) => Clight.External ef targs tres cc
+                  end)
+               _ _).
+Next Obligation. destruct a; auto. Qed.
+Next Obligation. destruct b; auto. destruct e. destruct p. destruct p. auto. Qed.
 Program Canonical Structure Fundef_common (fT:F Sig_signature): Fundef fT EF_external_function :=
-  mkFundef fT EF_external_function
-           (fun fd =>
-              match fd with
-                | AST.Internal f => inl f
-                | AST.External ef => inr ef
-              end) _.
-Next Obligation. destruct fd1, fd2; inv Hfd; auto. Qed.
+  @mkFundef _ fT EF_external_function (AST.fundef fT)
+            (mkEquivalentType
+               (fun fd =>
+                  match fd with
+                    | AST.Internal f => inl f
+                    | AST.External ef => inr ef
+                  end)
+               (fun fd =>
+                  match fd with
+                    | inl f => AST.Internal f
+                    | inr ef => AST.External ef
+                  end)
+               _ _).
+Next Obligation. destruct a; auto. Qed.
+Next Obligation. destruct b; auto. Qed.
 
 Canonical Structure V_type: V := mkV Ctypes.type_eq.
 Canonical Structure V_unit: V := mkV unit_eq.
 
 Canonical Structure Language_C: Language := mkLanguage Fundef_C V_type.
-Program Canonical Structure Language_ext_C: Language_ext :=
-  @mkLanguage_ext Language_C _ _
-                  (fun k fd args m => Csem.Callstate fd args k m)
-                  (fun k v m => Csem.Returnstate v k m)
-                  Csem.Kstop
-                  Cstrategy.step
-                  (Ctypes.Tfunction Ctypes.Tnil Ctypes.type_int32s cc_default) _ _ _.
-Next Obligation. intros [ge [evt [state' Hstep]]]. inv Hstep. inv H. inv H. Qed.
 
 Lemma Fundef_C_type_of_fundef f: Fundef_sig Fundef_C f = Csyntax.type_of_fundef f.
-Proof. unfold Fundef_sig, Fundef_dec. simpl. destruct f; auto. Qed.
-
-Lemma initial_state_C_equiv p s:
-  Language_ext_C.(initial_state) p s <-> Csem.initial_state p s.
-Proof.
-  constructor; intro X.
-  - destruct X as [a [f [m0 [Hm0 [Ha [Hf [Hsig ?]]]]]]]. simpl in *. subst.
-    econstructor; eauto. rewrite <- Fundef_C_type_of_fundef. auto.
-  - inv X. repeat eexists; eauto.
-    rewrite Fundef_C_type_of_fundef. auto.
-Qed.
-
-Lemma final_state_C_equiv s r:
-  Language_ext_C.(final_state) s r <-> Csem.final_state s r.
-Proof.
-  constructor; intro X; inv X; simpl in *; econstructor; simpl; eauto.
-Qed.
-
-Lemma c_sem_implies2 c:
-  forward_simulation (Cstrategy.semantics c) (Language_ext_C.(semantics) c).
-Proof.
-  apply semantics_compat; auto.
-  - intros. rewrite initial_state_C_equiv. constructor; auto.
-  - intros. rewrite final_state_C_equiv. constructor; auto.
-Qed.
-
+Proof. unfold Fundef_sig. destruct f; auto. Qed.
 
 Canonical Structure Language_Clight: Language := mkLanguage Fundef_Clight V_type.
-Program Canonical Structure Language_ext_Clight1: Language_ext :=
-  @mkLanguage_ext Language_Clight _ _
-                  (fun k fd args m => Clight.Callstate fd args k m)
-                  (fun k v m => Clight.Returnstate v k m)
-                  Clight.Kstop
-                  Clight.step1
-                  (Ctypes.Tfunction Ctypes.Tnil Ctypes.type_int32s cc_default) _ _ _.
-Next Obligation. intros [ge [evt [state' Hstep]]]. inv Hstep. Qed.
 
 Lemma Fundef_Clight_type_of_fundef f: Fundef_sig Fundef_Clight f = Clight.type_of_fundef f.
-Proof. unfold Fundef_sig, Fundef_dec. simpl. destruct f; auto. Qed.
-
-Lemma initial_state_Clight1_equiv p s:
-  Language_ext_Clight1.(initial_state) p s <-> Clight.initial_state p s.
-Proof.
-  constructor; intro X.
-  - destruct X as [a [f [m0 [Hm0 [Ha [Hf [Hsig ?]]]]]]]. simpl in *. subst.
-    econstructor; eauto. rewrite <- Fundef_Clight_type_of_fundef. auto.
-  - inv X. repeat eexists; eauto.
-    rewrite Fundef_Clight_type_of_fundef. auto.
-Qed.
-
-Lemma final_state_Clight1_equiv p r:
-  Language_ext_Clight1.(final_state) p r <-> Clight.final_state p r.
-Proof.
-  constructor; intro X; inv X; simpl in *; econstructor; simpl; eauto.
-Qed.
-
-Lemma clight1_sem_implies1 c:
-  forward_simulation (Language_ext_Clight1.(semantics) c) (Clight.semantics1 c).
-Proof.
-  apply semantics_compat; auto.
-  - intros. rewrite initial_state_Clight1_equiv. constructor; auto.
-  - intros. rewrite final_state_Clight1_equiv. constructor; auto.
-Qed.
-
-
-Program Canonical Structure Language_ext_Clight2: Language_ext :=
-  @mkLanguage_ext Language_Clight _ _
-                  (fun k fd args m => Clight.Callstate fd args k m)
-                  (fun k v m => Clight.Returnstate v k m)
-                  Clight.Kstop
-                  Clight.step2
-                  (Ctypes.Tfunction Ctypes.Tnil Ctypes.type_int32s cc_default) _ _ _.
-Next Obligation. intros [ge [evt [state' Hstep]]]. inv Hstep. Qed.
-
+Proof. unfold Fundef_sig. destruct f; auto. Qed.
 
 Canonical Structure Language_Csharpminor: Language := mkLanguage (Fundef_common F_Csharpminor) V_unit.
-Program Canonical Structure Language_ext_Csharpminor: Language_ext :=
-  @mkLanguage_ext Language_Csharpminor _ _
-                  (fun k fd args m => Csharpminor.Callstate fd args k m)
-                  (fun k v m => Csharpminor.Returnstate v k m)
-                  Csharpminor.Kstop
-                  Csharpminor.step
-                  AST.signature_main _ _ _.
-Next Obligation. intros [ge [evt [state' Hstep]]]. inv Hstep. Qed.
-
 
 Canonical Structure Language_Cminor: Language := mkLanguage (Fundef_common F_Cminor) V_unit.
-Program Canonical Structure Language_ext_Cminor: Language_ext :=
-  @mkLanguage_ext Language_Cminor _ _
-                  (fun k fd args m => Cminor.Callstate fd args k m)
-                  (fun k v m => Cminor.Returnstate v k m)
-                  Cminor.Kstop
-                  Cminor.step
-                  AST.signature_main _ _ _.
-Next Obligation. intros [ge [evt [state' Hstep]]]. inv Hstep. Qed.
 
 Lemma Fundef_Cminor_funsig f: Fundef_sig (Fundef_common F_Cminor) f = Cminor.funsig f.
-Proof. unfold Fundef_sig, Fundef_dec. simpl. destruct f; auto. Qed.
-
-Lemma initial_state_Cminor_equiv p s:
-  Language_ext_Cminor.(initial_state) p s <-> Cminor.initial_state p s.
-Proof.
-  constructor; intro X.
-  - destruct X as [a [f [m0 [Hm0 [Ha [Hf [Hsig ?]]]]]]]. simpl in *. subst.
-    econstructor; eauto. rewrite <- Fundef_Cminor_funsig. auto.
-  - inv X. repeat eexists; eauto.
-    rewrite Fundef_Cminor_funsig. auto.
-Qed.
-
-Lemma final_state_Cminor_equiv p r:
-  Language_ext_Cminor.(final_state) p r <-> Cminor.final_state p r.
-Proof.
-  constructor; intro X; inv X; simpl in *; econstructor; simpl; eauto.
-Qed.
-
-Lemma cminor_sem_implies2 rtl:
-  forward_simulation (Cminor.semantics rtl) (Language_ext_Cminor.(semantics) rtl).
-Proof.
-  apply semantics_compat; auto.
-  - intros. rewrite initial_state_Cminor_equiv. constructor; auto.
-  - intros. rewrite final_state_Cminor_equiv. constructor; auto.
-Qed.
-
+Proof. unfold Fundef_sig. destruct f; auto. Qed.
 
 Canonical Structure Language_CminorSel: Language := mkLanguage (Fundef_common F_CminorSel) V_unit.
-Program Canonical Structure Language_ext_CminorSel: Language_ext :=
-  @mkLanguage_ext Language_CminorSel _ _
-                  (fun k fd args m => CminorSel.Callstate fd args k m)
-                  (fun k v m => CminorSel.Returnstate v k m)
-                  CminorSel.Kstop
-                  CminorSel.step
-                  AST.signature_main _ _ _.
-Next Obligation. intros [ge [evt [state' Hstep]]]. inv Hstep. Qed.
 
 Lemma Fundef_CminorSel_funsig f: Fundef_sig (Fundef_common F_CminorSel) f = CminorSel.funsig f.
-Proof. unfold Fundef_sig, Fundef_dec. simpl. destruct f; auto. Qed.
-
-Lemma initial_state_CminorSel_equiv p s:
-  Language_ext_CminorSel.(initial_state) p s <-> CminorSel.initial_state p s.
-Proof.
-  constructor; intro X.
-  - destruct X as [a [f [m0 [Hm0 [Ha [Hf [Hsig ?]]]]]]]. simpl in *. subst.
-    econstructor; eauto. rewrite <- Fundef_CminorSel_funsig. auto.
-  - inv X. repeat eexists; eauto.
-    rewrite Fundef_CminorSel_funsig. auto.
-Qed.
-
-Lemma final_state_CminorSel_equiv p r:
-  Language_ext_CminorSel.(final_state) p r <-> CminorSel.final_state p r.
-Proof.
-  constructor; intro X; inv X; simpl in *; econstructor; simpl; eauto.
-Qed.
-
-Lemma cminorsel_sem_implies1 rtl:
-  forward_simulation (Language_ext_CminorSel.(semantics) rtl) (CminorSel.semantics rtl).
-Proof.
-  apply semantics_compat; auto.
-  - intros. rewrite initial_state_CminorSel_equiv. constructor; auto.
-  - intros. rewrite final_state_CminorSel_equiv. constructor; auto.
-Qed.
-
+Proof. unfold Fundef_sig. destruct f; auto. Qed.
 
 Canonical Structure Language_RTL: Language := mkLanguage (Fundef_common F_RTL) V_unit.
-Program Canonical Structure Language_ext_RTL: Language_ext :=
-  @mkLanguage_ext Language_RTL _ _
-                  RTL.Callstate
-                  RTL.Returnstate
-                  nil
-                  RTL.step
-                  AST.signature_main _ _ _.
-Next Obligation. intros [ge [evt [state' Hstep]]]. inv Hstep. Qed.
 
 Lemma Fundef_RTL_funsig f: Fundef_sig (Fundef_common F_RTL) f = RTL.funsig f.
-Proof. unfold Fundef_sig, Fundef_dec. simpl. destruct f; auto. Qed.
-
-Lemma initial_state_RTL_equiv p s:
-  Language_ext_RTL.(initial_state) p s <-> RTL.initial_state p s.
-Proof.
-  constructor; intro X.
-  - destruct X as [a [f [m0 [Hm0 [Ha [Hf [Hsig ?]]]]]]]. subst.
-    econstructor; eauto. rewrite <- Fundef_RTL_funsig. auto.
-  - inv X. repeat eexists; eauto.
-    rewrite Fundef_RTL_funsig. auto.
-Qed.
-
-Lemma final_state_RTL_equiv p r:
-  Language_ext_RTL.(final_state) p r <-> RTL.final_state p r.
-Proof.
-  constructor; intro X; inv X; simpl in *; econstructor; eauto.
-Qed.
-
-Lemma rtl_sem_implies1 rtl:
-  forward_simulation (Language_ext_RTL.(semantics) rtl) (RTL.semantics rtl).
-Proof.
-  apply semantics_compat; auto.
-  - intros. rewrite initial_state_RTL_equiv. constructor; auto.
-  - intros. rewrite final_state_RTL_equiv. constructor; auto.
-Qed.
-
-Lemma rtl_sem_implies2 rtl:
-  forward_simulation (RTL.semantics rtl) (Language_ext_RTL.(semantics) rtl).
-Proof.
-  apply semantics_compat; auto.
-  - intros. rewrite initial_state_RTL_equiv. constructor; auto.
-  - intros. rewrite final_state_RTL_equiv. constructor; auto.
-Qed.
-
+Proof. unfold Fundef_sig. destruct f; auto. Qed.
 
 Canonical Structure Language_LTL: Language := mkLanguage (Fundef_common F_LTL) V_unit.
 Canonical Structure Language_Linear: Language := mkLanguage (Fundef_common F_Linear) V_unit.
