sepcomp/common/SepcompRel.v
@@ -8,13 +8,75 @@ Require Import Errors.
 
 Set Implicit Arguments.
 
+Ltac clarify :=
+  repeat
+    match goal with
+      | [H: False |- _] => inv H
+      | [H1: ?x = _, H2: ?x = _ |- _] => rewrite H1 in H2; inv H2
+    end.
+
 Section SEPCOMP_RELATION.
 
 Variable (lang_src lang_tgt:Language).
-Variable grel:
+
+Variable transf_sigT: forall (ef:lang_src.(sigT)), lang_tgt.(sigT).
+Variable frel:
   forall (prog_src:lang_src.(progT))
-         (g_src:lang_src.(globdefT))
-         (g_tgt:lang_tgt.(globdefT)), Prop.
+         (f_src:lang_src.(fT))
+         (f_tgt:lang_tgt.(fT)), Prop.
+Variable transf_efT: forall (ef_src:lang_src.(efT)), res lang_tgt.(efT).
+Variable transf_vT: forall (v_src:lang_src.(vT)), res lang_tgt.(vT).
+
+Hypothesis frel_sigT:
+  forall p_src f_src f_tgt (H: frel p_src f_src f_tgt),
+    transf_sigT (lang_src.(fT).(F_sig) f_src) = lang_tgt.(fT).(F_sig) f_tgt.
+Hypothesis transf_efT_sigT:
+  forall ef_src ef_tgt (H: transf_efT ef_src = OK ef_tgt),
+    transf_sigT (lang_src.(efT).(EF_sig) ef_src) = lang_tgt.(efT).(EF_sig) ef_tgt.
+Hypothesis transf_efT_linkable:
+  forall ef_src ef_tgt (H: transf_efT ef_src = OK ef_tgt),
+    lang_src.(efT).(EF_linkable) ef_src = lang_tgt.(efT).(EF_linkable) ef_tgt.
+
+Inductive grel (prog_src:lang_src.(progT)):
+  forall (g_src:lang_src.(globdefT))
+         (g_tgt:lang_tgt.(globdefT)), Prop:=
+| grel_f
+    fd_src fd_tgt f_src f_tgt
+    (Hf_src: lang_src.(fundefT).(Fundef_equiv).(AtoB) fd_src = inl f_src)
+    (Hf_tgt: lang_tgt.(fundefT).(Fundef_equiv).(AtoB) fd_tgt = inl f_tgt)
+    (Hf: frel prog_src f_src f_tgt):
+    grel prog_src (Gfun fd_src) (Gfun fd_tgt)
+| grel_ef
+    fd_src fd_tgt ef_src ef_tgt
+    (Hef_src: lang_src.(fundefT).(Fundef_equiv).(AtoB) fd_src = inr ef_src)
+    (Hef_tgt: lang_tgt.(fundefT).(Fundef_equiv).(AtoB) fd_tgt = inr ef_tgt)
+    (Hef: transf_efT ef_src = OK ef_tgt):
+    grel prog_src (Gfun fd_src) (Gfun fd_tgt)
+| grel_gv
+    gv_src gv_tgt
+    (Hv: transf_globvar transf_vT gv_src = OK gv_tgt):
+    grel prog_src (Gvar gv_src) (Gvar gv_tgt)
+.
+
+Lemma linkable_grel_linkable
+      p1 g1 tg1 p2 g2 tg2
+      (Hg: globdef_linkable lang_src g1 g2)
+      (H1: grel p1 g1 tg1)
+      (H2: grel p2 g2 tg2):
+  globdef_linkable lang_tgt tg1 tg2.
+Proof.
+  inv H1; inv H2; inv Hg; inv Hv; clarify.
+  - constructor. econstructor; eauto.
+    + erewrite <- transf_efT_linkable; eauto.
+    + erewrite <- transf_efT_sigT; eauto.
+      erewrite <- frel_sigT; eauto.
+      rewrite Hsig. auto.
+  - constructor. eapply globfun_linkable_ee; eauto.
+  - inv Hv0. inv Hv1. monadInv H0. monadInv H1.
+    destruct gv_src, gv_src0. simpl in *. subst.
+    rewrite EQ in EQ0. inv EQ0.
+    constructor. constructor; auto.
+Qed.
 
 Section DEF.
 
@@ -38,6 +100,42 @@ End DEF.
 
 (** properties of linking on separate compilation relation *)
 
+Lemma list_forall2_PTree_unelements A B
+      (R:A->B->Prop) (p:list (ident*A)) (q:list (ident*B))
+      (H: list_forall2 (fun g1 g2 => fst g1 = fst g2 /\ R (snd g1) (snd g2)) p q):
+  PTree_rel
+    R
+    (PTree_unelements p)
+    (PTree_unelements q).
+Proof.
+  constructor. intro. rewrite ? PTree_guespec.
+  apply list_forall2_rev in H. revert H.
+  unfold ident in *. simpl in *. generalize (rev p) (rev q).
+  induction l; intros l0 H; inv H; simpl; auto.
+  destruct a. simpl. destruct (peq i p0); subst; simpl.
+  - destruct b1, H2 as [? ?]. simpl in *. subst.
+    destruct (peq p1 p1); simpl; [|xomega]. auto.
+  - destruct b1, H2 as [? ?]. simpl in *. subst.
+    destruct (peq i p1); simpl; [xomega|].
+    apply IHl. auto.
+Qed.
+
+Lemma PTree_rel_PTree_elements A B
+      (R:A->B->Prop) p q
+      (H: PTree_rel R p q):
+  list_forall2
+    (fun g1 g2 => fst g1 = fst g2 /\ R (snd g1) (snd g2))
+    (PTree.elements p) (PTree.elements q).
+Proof.
+  exploit (PTree.elements_canonical_order R p q).
+  - intros. inv H. specialize (H1 i). rewrite H0 in H1.
+    destruct (q ! i); [|inv H1]. eexists. split; auto.
+  - intros. inv H. specialize (H1 i). rewrite H0 in H1.
+    destruct (p ! i); [|inv H1]. eexists. split; auto.
+  - generalize (PTree.elements p) (PTree.elements q). clear p q H.
+    induction l; intros l0 X; inv X; constructor; auto.
+Qed.
+
 Lemma link_program_sepcomp_rel
       (prog1_src prog2_src prog_src:lang_src.(progT))
       (prog1_tgt prog2_tgt:lang_tgt.(progT))
@@ -48,6 +146,8 @@ Lemma link_program_sepcomp_rel
     link_program lang_tgt prog1_tgt prog2_tgt = Some prog_tgt /\
     sepcomp_rel prog_src prog_tgt.
 Proof.
+  exploit link_program_linkeq_l; eauto. intro Hle1.
+  exploit link_program_linkeq_r; eauto. intro Hle2.
   destruct prog1_src as [def1_src ?],
            prog2_src as [def2_src ?],
            prog_src as [def_src ?],
@@ -58,7 +158,101 @@ Proof.
   destruct (prog_main2 =? prog_main3)%positive eqn:Hmain; [|inv Hprog_src; fail].
   apply Peqb_true_eq in Hmain. subst.
   destruct (link_globdef_list lang_src def1_src def2_src) eqn:Hdef_src; inv Hprog_src.
-  admit.
+  apply (list_forall2_PTree_unelements
+           (fun g1 g2 =>
+              exists p,
+                program_linkeq lang_src p {| prog_defs := def1_src; prog_main := prog_main1 |} /\
+                grel p g1 g2)) in Hdefs.
+  apply (list_forall2_PTree_unelements
+           (fun g1 g2 =>
+              exists p,
+                program_linkeq lang_src p {| prog_defs := def2_src; prog_main := prog_main1 |} /\
+                grel p g1 g2)) in Hdefs0.
+  unfold link_globdef_list in *.
+  revert Hdefs Hdefs0 Hdef_src.
+  unfold globdefT. simpl.
+  repeat match goal with
+           | [|- context[@PTree_unelements ?T ?l]] => generalize (@PTree_unelements T l)
+         end.
+  intros def2'_tgt def2'_src def1'_tgt def1'_src H1 H2 Hsrc.
+  match goal with
+    | [H: context[match ?l with Some _ => _ | None => _ end] |- _] =>
+      destruct l as [defs_src|] eqn:Hdefs_src; inv H
+  end.
+  destruct (link_globdefs lang_tgt def1'_tgt def2'_tgt) as [defs_tgt|] eqn:Hdefs_tgt.
+  - eexists. split; eauto. constructor; simpl; auto.
+    apply
+      (@PTree_rel_PTree_elements _ _
+         (fun g1 g2 =>
+            exists p,
+              program_linkeq lang_src p {| prog_defs := PTree.elements defs_src; prog_main := prog_main1 |} /\
+              grel p g1 g2)).
+    constructor. intro.
+    eapply gtlink_globdefs in Hdefs_src. instantiate (1 := i) in Hdefs_src.
+    eapply gtlink_globdefs in Hdefs_tgt. instantiate (1 := i) in Hdefs_tgt.
+    inv H1. specialize (H i). inv H2. specialize (H0 i).
+    revert H H0 Hdefs_src Hdefs_tgt. unfold globdefT in *. simpl in *.
+    destruct (def1'_src ! i), (def1'_tgt ! i), (def2'_src ! i), (def2'_tgt ! i), (defs_src ! i), (defs_tgt ! i); intros H1 H2 H3 H4; subst; auto; clarify.
+    + destruct H3 as [[H3 ?]|[H3 ?]], H4 as [[H4 ?]|[H4 ?]]; subst.
+      * destruct H2 as [p [Hp Hg]]. eexists. split; [|eauto].
+        etransitivity; eauto.
+      * destruct H1 as [p1 [Hp1 H1]].
+        destruct H2 as [p2 [Hp2 H2]].
+        exploit linkable_grel_linkable; eauto. intro X.
+        inv H4; inv X.
+        { inv Hv; inv Hv0; clarify.
+          inv H1; inv H2; clarify.
+          eexists. split; [reflexivity|].
+          eapply grel_ef; eauto.
+        }
+        { inv H1. inv H2. monadInv Hv1. monadInv Hv2.
+          inv Hv. simpl in *. subst. inv Hv0. simpl in *.
+          destruct gv_src, gv_src0. simpl in *.
+          clear Hreadonly0 Hvolatile0. subst.
+          eexists. split; [reflexivity|].
+          eapply grel_gv; eauto.
+          unfold transf_globvar. simpl. rewrite EQ0. auto.
+        }
+      * destruct H1 as [p1 [Hp1 H1]].
+        destruct H2 as [p2 [Hp2 H2]].
+        exploit linkable_grel_linkable; eauto. intro X.
+        inv H4; inv X.
+        { inv Hv; inv Hv0; clarify.
+          inv H1; inv H2; clarify.
+          eexists. split; [reflexivity|].
+          eapply grel_ef; eauto.
+        }
+        { inv H1. inv H2. monadInv Hv1. monadInv Hv2.
+          inv Hv. simpl in *. subst. inv Hv0. simpl in *.
+          destruct gv_src, gv_src0. simpl in *.
+          clear Hreadonly0 Hvolatile0. subst.
+          eexists. split; [reflexivity|].
+          eapply grel_gv; eauto.
+          unfold transf_globvar. simpl. rewrite EQ. auto.
+        }
+      * destruct H1 as [p [Hp Hg]]. eexists. split; [|eauto].
+        etransitivity; eauto.
+    + destruct H1 as [p [Hp Hg]]. eexists. split; [|eauto].
+      etransitivity; eauto.
+    + destruct H2 as [p [Hp Hg]]. eexists. split; [|eauto].
+      etransitivity; eauto.
+  - apply gflink_globdefs in Hdefs_tgt. destruct Hdefs_tgt as [var [def1 [def2 [Hdef1 [Hdef2 [Hnl1 Hnl2]]]]]].
+    inv H1. specialize (H var). rewrite Hdef1 in H.
+    inv H2. specialize (H0 var). rewrite Hdef2 in H0.
+    eapply gtlink_globdefs in Hdefs_src. instantiate (1 := var) in Hdefs_src.
+    destruct (def1'_src ! var), (def2'_src ! var), (defs_src ! var);
+      try match goal with
+            | [H: False |- _] => inv H
+          end.
+    destruct Hdefs_src as [[Hl ?]|[Hl ?]]; subst.
+    + contradict Hnl1.
+      destruct H as [p1 [Hp1 H]].
+      destruct H0 as [p2 [Hp2 H0]].
+      eapply linkable_grel_linkable; eauto.
+    + contradict Hnl2.
+      destruct H as [p1 [Hp1 H]].
+      destruct H0 as [p2 [Hp2 H0]].
+      eapply linkable_grel_linkable; eauto.
 Qed.
 
 End SEPCOMP_RELATION.
@@ -79,31 +273,34 @@ Variable (vT_tgt:V).
 Let lang_src := mkLanguage fundefT_src vT_src.
 Let lang_tgt := mkLanguage fundefT_tgt vT_tgt.
 
-Variable transf_fun: lang_src.(progT) -> fundefT_src -> res fundefT_tgt.
-Variable transf_var: vT_src -> res vT_tgt.
+Variable transf_fT: lang_src.(progT) -> fT_src -> res fT_tgt.
+Variable transf_efT: efT_src -> res efT_tgt.
+Variable transf_vT: vT_src -> res vT_tgt.
+
+Let transf_fundefT (prog_src:lang_src.(progT)) (fd_src:fundefT_src): res fundefT_tgt :=
+  match fundefT_src.(Fundef_equiv).(AtoB) fd_src with
+    | inl f =>
+      bind
+        (transf_fT prog_src f)
+        (fun f => OK (fundefT_tgt.(Fundef_equiv).(BtoA) (inl f)))
+    | inr ef =>
+      bind
+        (transf_efT ef)
+        (fun ef => OK (fundefT_tgt.(Fundef_equiv).(BtoA) (inr ef)))
+  end.
+
 Variable p: lang_src.(progT).
 Variable p': lang_tgt.(progT).
 
-Inductive match_globdef_transf_partial2 (prog_src:lang_src.(progT)):
-  forall (def_src:lang_src.(globdefT))
-         (def_tgt:lang_tgt.(globdefT)), Prop :=
-| match_globdef_transf_partial2_fun
-    fun_src fun_tgt
-    (Hfun: transf_fun prog_src fun_src = OK fun_tgt):
-    match_globdef_transf_partial2 prog_src (Gfun fun_src) (Gfun fun_tgt)
-| match_globdef_transf_partial2_var
-    var_src var_tgt
-    (Hvar: transf_globvar transf_var var_src = OK var_tgt):
-    match_globdef_transf_partial2 prog_src (Gvar var_src) (Gvar var_tgt)
-.
-
 Section TRANSF.
 
-Hypothesis TRANSF: transform_partial_program2 (transf_fun p) transf_var p = OK p'.
+Hypothesis TRANSF: transform_partial_program2 (transf_fundefT p) transf_vT p = OK p'.
 
 Lemma transf_partial2_sepcomp_rel:
-  sepcomp_rel
-    match_globdef_transf_partial2
+  @sepcomp_rel
+    lang_src lang_tgt
+    (fun p f tf => transf_fT p f = OK tf)
+    transf_efT transf_vT
     p p'.
 Proof.
   destruct p as [defs ?], p' as [tdefs ?].
@@ -119,7 +316,9 @@ Proof.
     end.
     monadInv Hdefs. constructor; simpl.
     + split; auto. eexists. split; [reflexivity|].
-      constructor. auto.
+      unfold transf_fundefT in Hf. destruct (fundefT_src.(AtoB) f) as [func|efunc] eqn:Hf'; monadInv Hf.
+      * eapply grel_f; eauto. apply HBAB.
+      * eapply grel_ef; eauto. apply HBAB.
     + apply IHdefs. auto.
   - match goal with
       | [H: match ?x with OK _ => _ | Error _ => _ end = OK _ |- _] =>
@@ -135,16 +334,20 @@ End TRANSF.
 
 Section INITIAL.
 
-Hypothesis Hsepcomp_rel: sepcomp_rel match_globdef_transf_partial2 p p'.
+Hypothesis Hsepcomp_rel:
+  @sepcomp_rel
+    lang_src lang_tgt
+    (fun p f tf => transf_fT p f = OK tf)
+    transf_efT transf_vT
+    p p'.
 
-Lemma prog_match:
+Let prog_match:
   match_program
     (fun fd tfd =>
        exists prog_src,
          program_linkeq lang_src prog_src p /\
-         transf_fun prog_src fd = OK tfd)
-    (fun info tinfo =>
-       transf_var info = OK tinfo)
+         transf_fundefT prog_src fd = OK tfd)
+    (fun info tinfo => transf_vT info = OK tinfo)
     nil p.(prog_main)
     p p'.
 Proof.
@@ -161,7 +364,12 @@ Proof.
   constructor; auto.
   destruct H1 as [prog_src [Hprog_src H1]]. inv H1.
   - apply match_glob_fun. eexists. split; eauto.
-  - monadInv Hvar. destruct var_src. simpl in *.
+    unfold transf_fundefT. simpl in *.
+    rewrite Hf_src, Hf. simpl. rewrite <- Hf_tgt, HABA. auto.
+  - apply match_glob_fun. eexists. split; eauto.
+    unfold transf_fundefT. simpl in *.
+    rewrite Hef_src, Hef. simpl. rewrite <- Hef_tgt, HABA. auto.
+  - unfold transf_globvar in Hv. monadInv Hv. simpl in *. destruct gv_src.
     apply match_glob_var. auto.
 Qed.
 
@@ -172,7 +380,7 @@ Theorem find_funct_ptr_transf_partial2:
   Genv.find_funct_ptr (Genv.globalenv p') b = Some f' /\ 
   exists prog_src,
     program_linkeq lang_src prog_src p /\
-    transf_fun prog_src f = OK f'.
+    transf_fundefT prog_src f = OK f'.
 Proof.
   intros. 
   exploit Genv.find_funct_ptr_match. eexact prog_match. eauto. 
@@ -185,7 +393,7 @@ Theorem find_funct_ptr_rev_transf_partial2:
   exists f, Genv.find_funct_ptr (Genv.globalenv p) b = Some f /\ 
   exists prog_src,
     program_linkeq lang_src prog_src p /\
-    transf_fun prog_src f = OK tf.
+    transf_fundefT prog_src f = OK tf.
 Proof.
   intros. 
   exploit Genv.find_funct_ptr_rev_match. eexact prog_match. eauto. 
@@ -200,7 +408,7 @@ Theorem find_funct_transf_partial2:
   Genv.find_funct (Genv.globalenv p') v = Some f' /\ 
   exists prog_src,
     program_linkeq lang_src prog_src p /\
-    transf_fun prog_src f = OK f'.
+    transf_fundefT prog_src f = OK f'.
 Proof.
   intros. 
   exploit Genv.find_funct_match. eexact prog_match. eauto. 
@@ -213,7 +421,7 @@ Theorem find_funct_rev_transf_partial2:
   exists f, Genv.find_funct (Genv.globalenv p) v = Some f /\ 
   exists prog_src,
     program_linkeq lang_src prog_src p /\
-    transf_fun prog_src f = OK tf.
+    transf_fundefT prog_src f = OK tf.
 Proof.
   intros. 
   exploit Genv.find_funct_rev_match. eexact prog_match. eauto. 
@@ -224,7 +432,7 @@ Theorem find_var_info_transf_partial2:
   forall (b: block) (v: globvar vT_src),
   Genv.find_var_info (Genv.globalenv p) b = Some v ->
   exists v',
-  Genv.find_var_info (Genv.globalenv p') b = Some v' /\ transf_globvar transf_var v = OK v'.
+  Genv.find_var_info (Genv.globalenv p') b = Some v' /\ transf_globvar transf_vT v = OK v'.
 Proof.
   intros. 
   exploit Genv.find_var_info_match. eexact prog_match. eauto. intros [tv [X Y]]. 
@@ -236,7 +444,7 @@ Theorem find_var_info_rev_transf_partial2:
   forall (b: block) (v': globvar vT_tgt),
   Genv.find_var_info (Genv.globalenv p') b = Some v' ->
   exists v,
-  Genv.find_var_info (Genv.globalenv p) b = Some v /\ transf_globvar transf_var v = OK v'.
+  Genv.find_var_info (Genv.globalenv p) b = Some v /\ transf_globvar transf_vT v = OK v'.
 Proof.
   intros. 
   exploit Genv.find_var_info_rev_match. eexact prog_match. eauto.
@@ -255,9 +463,7 @@ Qed.
 Theorem init_mem_transf_partial2:
   forall m, Genv.init_mem p = Some m -> Genv.init_mem p' = Some m.
 Proof.
-  intros. erewrite Genv.init_mem_match; eauto.
-  instantiate (1 := nil). eauto.
-  eexact prog_match. auto.
+  intros. erewrite Genv.init_mem_match; eauto. eauto.
 Qed.
 
 End INITIAL.
@@ -279,55 +485,48 @@ Variable (vT:V).
 Let lang_src := mkLanguage fundefT_src vT.
 Let lang_tgt := mkLanguage fundefT_tgt vT.
 
-Variable transf: lang_src.(progT) -> fundefT_src -> res fundefT_tgt.
+Variable transf_fT: lang_src.(progT) -> fT_src -> res fT_tgt.
+Variable transf_efT: efT_src -> res efT_tgt.
+
+Let transf_fundefT (prog_src:lang_src.(progT)) (fd_src:fundefT_src): res fundefT_tgt :=
+  match fundefT_src.(Fundef_equiv).(AtoB) fd_src with
+    | inl f =>
+      bind
+        (transf_fT prog_src f)
+        (fun f => OK (fundefT_tgt.(Fundef_equiv).(BtoA) (inl f)))
+    | inr ef =>
+      bind
+        (transf_efT ef)
+        (fun ef => OK (fundefT_tgt.(Fundef_equiv).(BtoA) (inr ef)))
+  end.
+
 Variable p: lang_src.(progT).
 Variable p': lang_tgt.(progT).
 
-Inductive match_globdef_transf_partial (prog_src:lang_src.(progT)):
-  forall (def_src:lang_src.(globdefT))
-         (def_tgt:lang_tgt.(globdefT)), Prop :=
-| match_globdef_transf_partial_fun
-    fun_src fun_tgt
-    (Hfun: transf prog_src fun_src = OK fun_tgt):
-    match_globdef_transf_partial prog_src (Gfun fun_src) (Gfun fun_tgt)
-| match_globdef_transf_partial_var var:
-    match_globdef_transf_partial prog_src (Gvar var) (Gvar var)
-.
-
 Section TRANSF.
 
-Hypothesis TRANSF: transform_partial_program (transf p) p = OK p'.
+Hypothesis TRANSF: transform_partial_program (transf_fundefT p) p = OK p'.
 
 Lemma transf_partial_sepcomp_rel:
-  sepcomp_rel
-    match_globdef_transf_partial
+  @sepcomp_rel
+    lang_src lang_tgt
+    (fun p f tf => transf_fT p f = OK tf)
+    transf_efT (@OK _)
     p p'.
 Proof.
-  exploit transf_partial2_sepcomp_rel; eauto. intro X.
-  inv X. constructor; auto.
-  eapply list_forall2_imply; eauto. simpl. intros.
-  destruct v1, v2, H1 as [? [sp [Hsp Hmatch]]]. simpl in *. subst.
-  split; auto. eexists. split; eauto.
-  inv Hmatch.
-  - constructor. auto.
-  - monadInv Hvar. inv EQ. destruct var_src. constructor.
+  exploit transf_partial2_sepcomp_rel; eauto.
 Qed.
 
 End TRANSF.
 
 Section INITIAL.
 
-Hypothesis Hsepcomp_rel: sepcomp_rel match_globdef_transf_partial p p'.
-
-Let transf_OK:
-  sepcomp_rel (match_globdef_transf_partial2 transf (fun v => OK v)) p p'.
-Proof.
-  inv Hsepcomp_rel. constructor; auto.
-  eapply list_forall2_imply; eauto. simpl. intros.
-  destruct v1, v2, H1 as [? [prog_src [Hprog_src X]]]. simpl in *. subst.
-  split; auto. eexists. split; eauto.
-  inv X; constructor; auto. destruct var. auto.
-Qed.
+Hypothesis Hsepcomp_rel:
+  @sepcomp_rel
+    lang_src lang_tgt
+    (fun p f tf => transf_fT p f = OK tf)
+    transf_efT (@OK _)
+    p p'.
 
 Theorem find_funct_ptr_transf_partial:
   forall (b: block) (f: fundefT_src),
@@ -336,8 +535,8 @@ Theorem find_funct_ptr_transf_partial:
   Genv.find_funct_ptr (Genv.globalenv p') b = Some f' /\ 
   exists prog_src,
     program_linkeq lang_src prog_src p /\
-    transf prog_src f = OK f'.
-Proof (find_funct_ptr_transf_partial2 transf_OK).
+    transf_fundefT prog_src f = OK f'.
+Proof (find_funct_ptr_transf_partial2 _ Hsepcomp_rel).
 
 Theorem find_funct_ptr_rev_transf_partial:
   forall (b: block) (tf: fundefT_tgt),
@@ -345,8 +544,8 @@ Theorem find_funct_ptr_rev_transf_partial:
   exists f, Genv.find_funct_ptr (Genv.globalenv p) b = Some f /\ 
   exists prog_src,
     program_linkeq lang_src prog_src p /\
-    transf prog_src f = OK tf.
-Proof (find_funct_ptr_rev_transf_partial2 transf_OK).
+    transf_fundefT prog_src f = OK tf.
+Proof (find_funct_ptr_rev_transf_partial2 _ Hsepcomp_rel).
 
 Theorem find_funct_transf_partial:
   forall (v: val) (f: fundefT_src),
@@ -355,8 +554,8 @@ Theorem find_funct_transf_partial:
   Genv.find_funct (Genv.globalenv p') v = Some f' /\ 
   exists prog_src,
     program_linkeq lang_src prog_src p /\
-    transf prog_src f = OK f'.
-Proof (find_funct_transf_partial2 transf_OK).
+    transf_fundefT prog_src f = OK f'.
+Proof (find_funct_transf_partial2 _ Hsepcomp_rel).
 
 Theorem find_funct_rev_transf_partial:
   forall (v: val) (tf: fundefT_tgt),
@@ -364,18 +563,18 @@ Theorem find_funct_rev_transf_partial:
   exists f, Genv.find_funct (Genv.globalenv p) v = Some f /\ 
   exists prog_src,
     program_linkeq lang_src prog_src p /\
-    transf prog_src f = OK tf.
-Proof (find_funct_rev_transf_partial2 transf_OK).
+    transf_fundefT prog_src f = OK tf.
+Proof (find_funct_rev_transf_partial2 _ Hsepcomp_rel).
 
 Theorem find_var_info_transf_partial:
   forall (b: block),
   Genv.find_var_info (Genv.globalenv p') b = Genv.find_var_info (Genv.globalenv p) b.
 Proof.
   intros. destruct (Genv.find_var_info (Genv.globalenv p) b) as [v|] eqn:Hg.
-  - exploit find_var_info_transf_partial2; try apply transf_OK; eauto.
+  - exploit find_var_info_transf_partial2; try apply Hsepcomp_rel; eauto.
     simpl. intros [v'' [Hv'' X]]. destruct v. inv X. auto.
   - destruct (Genv.find_var_info (Genv.globalenv p') b) as [v|] eqn:Hg'; [|auto].
-    exploit find_var_info_rev_transf_partial2; try apply transf_OK; eauto.
+    exploit find_var_info_rev_transf_partial2; try apply Hsepcomp_rel; eauto.
     simpl. intros [v'' [Hv'' X]].
     simpl in *. rewrite Hg in Hv''. inv Hv''.
 Qed.
@@ -383,11 +582,11 @@ Qed.
 Theorem find_symbol_transf_partial:
   forall (s: ident),
   Genv.find_symbol (Genv.globalenv p') s = Genv.find_symbol (Genv.globalenv p) s.
-Proof (find_symbol_transf_partial2 transf_OK).
+Proof (find_symbol_transf_partial2 _ Hsepcomp_rel).
 
 Theorem init_mem_transf_partial:
   forall m, Genv.init_mem p = Some m -> Genv.init_mem p' = Some m.
-Proof (init_mem_transf_partial2 transf_OK).
+Proof (init_mem_transf_partial2 _ Hsepcomp_rel).
 
 End INITIAL.
 
@@ -408,28 +607,29 @@ Variable (vT:V).
 Let lang_src := mkLanguage fundefT_src vT.
 Let lang_tgt := mkLanguage fundefT_tgt vT.
 
-Variable transf: lang_src.(progT) -> fundefT_src -> fundefT_tgt.
+Variable transf_fT: lang_src.(progT) -> fT_src -> fT_tgt.
+Variable transf_efT: efT_src -> efT_tgt.
+
+Let transf_fundefT (prog_src:lang_src.(progT)) (fd_src:fundefT_src): fundefT_tgt :=
+  match fundefT_src.(Fundef_equiv).(AtoB) fd_src with
+    | inl f =>
+      fundefT_tgt.(Fundef_equiv).(BtoA) (inl (transf_fT prog_src f))
+    | inr ef =>
+      fundefT_tgt.(Fundef_equiv).(BtoA) (inr (transf_efT ef))
+  end.
+
 Variable p: lang_src.(progT).
 Variable tp: lang_tgt.(progT).
 
-Inductive match_globdef_transf_program (prog_src:lang_src.(progT)):
-  forall (def_src:lang_src.(globdefT))
-         (def_tgt:lang_tgt.(globdefT)), Prop :=
-| match_globdef_transf_program_fun
-    fun_src fun_tgt
-    (Hfun: transf prog_src fun_src = fun_tgt):
-    match_globdef_transf_program prog_src (Gfun fun_src) (Gfun fun_tgt)
-| match_globdef_transf_program_var var:
-    match_globdef_transf_program prog_src (Gvar var) (Gvar var)
-.
-
 Section TRANSF.
 
-Hypothesis TRANSF: transform_program (transf p) p = tp.
+Hypothesis TRANSF: transform_program (transf_fundefT p) p = tp.
 
 Lemma transf_program_sepcomp_rel:
-  sepcomp_rel
-    match_globdef_transf_program
+  @sepcomp_rel
+    lang_src lang_tgt
+    (fun p f tf => transf_fT p f = tf)
+    (fun ef => OK (transf_efT ef)) (@OK _)
     p tp.
 Proof.
   destruct p as [defs ?], tp as [tdefs ?]. inv TRANSF.
@@ -440,8 +640,10 @@ Proof.
     + destruct a. destruct g; auto.
     + eexists. split; [reflexivity|].
       destruct a. simpl. destruct g.
-      * constructor. auto.
-      * constructor.
+      * unfold transf_fundefT. destruct (fundefT_src.(AtoB) f) as [func|efunc] eqn:Hf'.
+        { eapply grel_f; eauto. apply HBAB. }
+        { eapply grel_ef; eauto. apply HBAB. }
+      * constructor. destruct v. auto.
   - apply IHdefs.
 Qed.
 
@@ -449,19 +651,44 @@ End TRANSF.
 
 Section INITIAL.
 
-Hypothesis Hsepcomp_rel: sepcomp_rel match_globdef_transf_program p tp.
+Hypothesis Hsepcomp_rel:
+  @sepcomp_rel
+    lang_src lang_tgt
+    (fun p f tf => transf_fT p f = tf)
+    (fun ef => OK (transf_efT ef)) (@OK _)
+    p tp.
 
-Let transf_OK:
-  sepcomp_rel (match_globdef_transf_partial2 (fun p x => OK (transf p x)) (fun v => OK v)) p tp.
+Let prog_match:
+  match_program
+    (fun fd tfd =>
+       exists prog_src,
+         program_linkeq lang_src prog_src p /\
+         transf_fundefT prog_src fd = tfd)
+    (fun info tinfo => info = tinfo)
+    nil p.(prog_main)
+    p tp.
 Proof.
-  inv Hsepcomp_rel. constructor; auto.
-  eapply list_forall2_imply; eauto.
-  simpl. intros. destruct v1, v2, H1 as [? X]. simpl in *. subst.
-  destruct X as [prog_src [Hprog_src Hg]].
-  split; auto. eexists. split; eauto.
-  inv Hg.
-  - constructor. auto.
-  - constructor. destruct var. auto.
+  destruct p as [defs ?], tp as [defs' ?].
+  inv Hsepcomp_rel. simpl in *. subst.
+  revert defs' Hdefs. generalize defs at 1 3 as fdefs.
+  induction defs; intros fdefs defs' Hdefs.
+  { inv Hdefs. constructor; auto. exists nil. split; auto. constructor. }
+  inv Hdefs. destruct a, b1, H1 as [? H1]. simpl in *. subst.
+  eapply IHdefs in H3. destruct H3 as [H3 ?]. split; [|auto].
+  destruct H3 as [? H3]. simpl in *. rewrite app_nil_r in *.
+  destruct H3 as [H3 ?]. subst.
+  eexists. rewrite app_nil_r. split; auto.
+  constructor; auto.
+  destruct H1 as [prog_src [Hprog_src H1]]. inv H1.
+  - apply match_glob_fun. eexists. split; eauto.
+    unfold transf_fundefT. simpl in *.
+    rewrite Hf_src, <- Hf_tgt. apply HABA.
+  - apply match_glob_fun. eexists. split; eauto. inv Hef.
+    unfold transf_fundefT. simpl in *.
+    rewrite Hef_src, <- Hef_tgt. apply HABA.
+  - unfold transf_globvar in Hv. monadInv Hv. inv EQ.
+    simpl in *. destruct gv_src.
+    apply match_glob_var. auto.
 Qed.
 
 Theorem find_funct_ptr_transf:
@@ -469,12 +696,12 @@ Theorem find_funct_ptr_transf:
   Genv.find_funct_ptr (Genv.globalenv p) b = Some f ->
   exists prog_src,
     program_linkeq lang_src prog_src p /\
-    Genv.find_funct_ptr (Genv.globalenv tp) b = Some (transf prog_src f).
+    Genv.find_funct_ptr (Genv.globalenv tp) b = Some (transf_fundefT prog_src f).
 Proof.
   intros. 
-  destruct (@find_funct_ptr_transf_partial2 _ _ _ _ _ _ _ _ _ _ _ _ _ _ transf_OK _ _ H)
-  as [f' [X [prog_src [Hprog_src Y]]]]. 
-  simpl in *. eexists. split; eauto. congruence.
+  exploit Genv.find_funct_ptr_match. eexact prog_match. eauto. 
+  intros [tf [X [prog_src [Hprog_src Y]]]]. subst.
+  eexists. split; eauto.
 Qed.
 
 Theorem find_funct_ptr_rev_transf:
@@ -483,11 +710,12 @@ Theorem find_funct_ptr_rev_transf:
   exists f, Genv.find_funct_ptr (Genv.globalenv p) b = Some f /\
             exists prog_src,
               program_linkeq lang_src prog_src p /\
-              transf prog_src f = tf.
+              transf_fundefT prog_src f = tf.
 Proof.
-  intros. exploit find_funct_ptr_rev_transf_partial2. eexact transf_OK. eauto.
-  intros [f [X [prog_src [Hprog_src Y]]]]. exists f; split. auto. 
-  eexists. split; eauto. congruence.
+  intros. 
+  exploit Genv.find_funct_ptr_rev_match. eexact prog_match. eauto. 
+  destruct (plt b (Genv.genv_next (Genv.globalenv p))); [|intro X; inv X].
+  intros [f [X Y]]. exists f; auto.
 Qed.
 
 Theorem find_funct_transf:
@@ -495,12 +723,12 @@ Theorem find_funct_transf:
   Genv.find_funct (Genv.globalenv p) v = Some f ->
   exists prog_src,
     program_linkeq lang_src prog_src p /\
-    Genv.find_funct (Genv.globalenv tp) v = Some (transf prog_src f).
+    Genv.find_funct (Genv.globalenv tp) v = Some (transf_fundefT prog_src f).
 Proof.
   intros. 
-  destruct (@find_funct_transf_partial2 _ _ _ _ _ _ _ _ _ _ _ _ _ _ transf_OK _ _ H)
-  as [f' [X [prog_src [Hprog_src Y]]]]. 
-  eexists. split; eauto. simpl in *. congruence.
+  exploit Genv.find_funct_match. eexact prog_match. eauto. 
+  intros [tf [X [prog_src [Hprog_src Y]]]]. subst.
+  eexists. split; eauto.
 Qed.
 
 Theorem find_funct_rev_transf:
@@ -509,18 +737,18 @@ Theorem find_funct_rev_transf:
   exists f, Genv.find_funct (Genv.globalenv p) v = Some f /\ 
             exists prog_src,
               program_linkeq lang_src prog_src p /\
-              transf prog_src f = tf.
+              transf_fundefT prog_src f = tf.
 Proof.
-  intros. exploit find_funct_rev_transf_partial2. eexact transf_OK. eauto.
-  intros [f [X [prog_src [Hprog_src Y]]]]. exists f; split. auto. 
-  eexists. split; eauto. congruence.
+  intros. 
+  exploit Genv.find_funct_rev_match. eexact prog_match. eauto. 
+  intros [[f [X Y]]|X]; [|inv X]. exists f; auto.
 Qed.
 
 Theorem find_symbol_transf:
   forall (s: ident),
   Genv.find_symbol (Genv.globalenv tp) s = Genv.find_symbol (Genv.globalenv p) s.
 Proof.
-  exact (@find_symbol_transf_partial2 _ _ _ _ _ _ _ _ _ _ _ _ _ _ transf_OK).
+  intros. eapply Genv.find_symbol_match. eexact prog_match. auto.
 Qed.
 
 Theorem find_var_info_transf:
@@ -528,18 +756,18 @@ Theorem find_var_info_transf:
   Genv.find_var_info (Genv.globalenv tp) b = Genv.find_var_info (Genv.globalenv p) b.
 Proof.
   intros. destruct (Genv.find_var_info (Genv.globalenv p) b) as [v|] eqn:Hg.
-  - exploit find_var_info_transf_partial2; try apply transf_OK; eauto.
-    simpl. intros [v' [Hv' X]]. destruct v. inv X. auto.
+  - exploit Genv.find_var_info_match. eexact prog_match. eauto. intros [tv [X Y]].
+    inv Y. auto.
   - destruct (Genv.find_var_info (Genv.globalenv tp) b) as [v|] eqn:Hg'; [|auto].
-    exploit find_var_info_rev_transf_partial2; try apply transf_OK; eauto.
-    simpl. intros [v' [Hv' X]].
-    simpl in *. rewrite Hg in Hv'. inv Hv'.
+    exploit Genv.find_var_info_rev_match. eexact prog_match. eauto.
+    destruct (plt b (Genv.genv_next (Genv.globalenv p))); [|intro X; inv X].
+    intros [v' [X Y]]. rewrite Hg in X. inv X.
 Qed.
 
 Theorem init_mem_transf:
   forall m, Genv.init_mem p = Some m -> Genv.init_mem tp = Some m.
 Proof.
-  exact (@init_mem_transf_partial2 _ _ _ _ _ _ _ _ _ _ _ _ _ _ transf_OK).
+  intros. erewrite Genv.init_mem_match; eauto. eauto.
 Qed.
 
 End INITIAL.
