sepcomp/backend/Constpropproof_sepcomp.v
@@ -45,13 +45,8 @@ Variable tprog: program.
 Hypothesis TRANSF:
   @sepcomp_rel
     Language_RTL Language_RTL
-    (@match_globdef_transf_program
-       Sig_signature Sig_signature
-       F_RTL F_RTL
-       EF_external_function EF_external_function
-       (Fundef_common F_RTL) (Fundef_common F_RTL)
-       V_unit
-       (fun p f => transf_fundef (romem_for_program p) f))
+    (fun p f tf => transf_function (romem_for_program p) f = tf)
+    (@Errors.OK _) (@Errors.OK _)
     prog tprog.
 Let ge := Genv.globalenv prog.
 Let tge := Genv.globalenv tprog.
@@ -64,11 +59,11 @@ Let rm := romem_for_program prog.
 
 Lemma symbols_preserved:
   forall (s: ident), Genv.find_symbol tge s = Genv.find_symbol ge s.
-Proof (find_symbol_transf TRANSF).
+Proof (find_symbol_transf _ _ TRANSF).
 
 Lemma varinfo_preserved:
   forall b, Genv.find_var_info tge b = Genv.find_var_info ge b.
-Proof (find_var_info_transf TRANSF).
+Proof (find_var_info_transf _ _ TRANSF).
 
 Lemma functions_translated:
   forall (v: val) (f: fundef),
@@ -76,7 +71,12 @@ Lemma functions_translated:
   exists sprog,
     program_linkeq Language_RTL sprog prog /\
     Genv.find_funct tge v = Some (transf_fundef (romem_for_program sprog) f).
-Proof (find_funct_transf TRANSF).
+Proof.
+  intros. exploit (find_funct_transf _ _ TRANSF); eauto. simpl in *.
+  intros [sprog [Hsprog Hf]].
+  eexists. split; eauto.
+  destruct f; auto.
+Qed.
 
 Lemma function_ptr_translated:
   forall (b: block) (f: fundef),
@@ -84,7 +84,12 @@ Lemma function_ptr_translated:
   exists sprog,
     program_linkeq Language_RTL sprog prog /\
     Genv.find_funct_ptr tge b = Some (transf_fundef (romem_for_program sprog) f).
-Proof (find_funct_ptr_transf TRANSF).
+Proof.
+  intros. exploit (find_funct_ptr_transf _ _ TRANSF); eauto. simpl in *.
+  intros [sprog [Hsprog Hf]].
+  eexists. split; eauto.
+  destruct f; auto.
+Qed.
 
 Lemma sig_function_translated:
   forall rm f,
@@ -619,7 +624,7 @@ Proof.
   exploit function_ptr_translated; eauto. intros [sprog [Hsprog FIND]].
   exists O; exists (Callstate nil (transf_fundef (romem_for_program sprog) f) nil m0); split.
   econstructor; eauto.
-  apply (init_mem_transf TRANSF); auto.
+  apply (init_mem_transf _ _ TRANSF); auto.
   replace (prog_main tprog) with (prog_main prog).
   rewrite symbols_preserved. eauto.
   inv TRANSF. auto.
