sepcomp/backend/Tailcallproof_sepcomp.v
@@ -242,37 +242,33 @@ Variable tprog: program.
 Hypothesis TRANSF:
   @sepcomp_rel
     Language_RTL Language_RTL
-    (@match_globdef_transf_program
-       Sig_signature Sig_signature
-       F_RTL F_RTL
-       EF_external_function EF_external_function
-       (Fundef_common F_RTL) (Fundef_common F_RTL)
-       V_unit
-       (fun p f => transf_fundef f))
+    (fun p f tf => transf_function f = tf)
+    (@Errors.OK _) (@Errors.OK _)
     prog tprog.
 Let ge := Genv.globalenv prog.
 Let tge := Genv.globalenv tprog.
 
 Lemma symbols_preserved:
   forall (s: ident), Genv.find_symbol tge s = Genv.find_symbol ge s.
-Proof (find_symbol_transf TRANSF). 
+Proof (find_symbol_transf _ _ TRANSF). 
 
 Lemma varinfo_preserved:
   forall b, Genv.find_var_info tge b = Genv.find_var_info ge b.
-Proof (find_var_info_transf TRANSF).
+Proof (find_var_info_transf _ _ TRANSF).
 
 Lemma functions_translated:
   forall (v: val) (f: RTL.fundef),
   Genv.find_funct ge v = Some f ->
   Genv.find_funct tge v = Some (transf_fundef f).
 Proof.
-  generalize (find_funct_transf TRANSF).
+  generalize (find_funct_transf _ _ TRANSF).
   intros H1 v f. specialize (H1 v f).
   revert H1. unfold ge, fundef. simpl.
   match goal with
     | [|- _ -> ?a = _ -> _] => destruct a
   end; intros H1 H2; inv H2.
-  specialize (H1 eq_refl). destruct H1 as [? [? H1]]. auto.
+  specialize (H1 eq_refl). destruct H1 as [? [? H1]].
+  destruct f; auto.
 Qed.
 
 Lemma funct_ptr_translated:
@@ -280,13 +276,14 @@ Lemma funct_ptr_translated:
   Genv.find_funct_ptr ge b = Some f ->
   Genv.find_funct_ptr tge b = Some (transf_fundef f).
 Proof.
-  generalize (find_funct_ptr_transf TRANSF).
+  generalize (find_funct_ptr_transf _ _ TRANSF).
   intros H1 v f. specialize (H1 v f).
   revert H1. unfold ge, fundef. simpl.
   match goal with
     | [|- _ -> ?a = _ -> _] => destruct a
   end; intros H1 H2; inv H2.
-  specialize (H1 eq_refl). destruct H1 as [? [? H1]]. auto.
+  specialize (H1 eq_refl). destruct H1 as [? [? H1]].
+  destruct f; auto.
 Qed.
 
 Lemma sig_preserved:
@@ -625,7 +622,7 @@ Proof.
   intros. inv H. 
   exploit funct_ptr_translated; eauto. intro FIND.
   exists (Callstate nil (transf_fundef f) nil m0); split.
-  econstructor; eauto. apply (init_mem_transf TRANSF). auto.
+  econstructor; eauto. apply (init_mem_transf _ _ TRANSF). auto.
   replace (prog_main tprog) with (prog_main prog).
   rewrite symbols_preserved. eauto.
   inv TRANSF. auto.
